src/riot/RIoT.X509.AliasKeyTBS.fsti
@@ -258,7 +258,7 @@ let x509_get_AliasKeyTBS
   (s_org:     x509_RDN_x520_attribute_string_t ORGANIZATION IA5_STRING)
   (s_country: x509_RDN_x520_attribute_string_t COUNTRY      PRINTABLE_STRING)
   (ku: key_usage_payload_t)
-  (keyID: datatype_of_asn1_type OCTET_STRING { dfst keyID == 20ul })
+  (keyID: datatype_of_asn1_type OCTET_STRING { keyID.ASN1.Base.len == 20ul })
   (version: datatype_of_asn1_type INTEGER)
   (fwid: B32.lbytes32 32ul)
   (deviceIDPub: B32.lbytes32 32ul)
